big refactoring

lawyer/nonblocking/trace_context.v
@@ -1,6 +1,6 @@
 From trillium.traces Require Import exec_traces trace_lookup. 
 From trillium.program_logic Require Import language adequacy.
-From fairness Require Import locales_helpers. 
+From fairness Require Import locales_helpers utils. 
 
 
 Section ThreadPoolContext.
@@ -59,7 +59,62 @@ Section ThreadPoolContext.
     red. eexists. split; eauto.
   Qed.
 
+  Lemma no_expr_in_empty_pool κ σ e:
+    ¬ expr_at κ ([], σ) e.
+  Proof using. destruct κ. rewrite /expr_at. set_solver. Qed. 
+
+  (* TODO: use in more places *)
+  Lemma nval_enabled K τ c
+    (NVAL: nval_at (TpoolCtx K τ) c):
+    locale_enabled τ c.
+  Proof using. 
+    red. red in NVAL. simpl in NVAL. destruct NVAL as (?&?&?).
+    eexists. split; eauto.
+    eapply fill_not_val; eauto.
+  Qed.
+
 End ThreadPoolContext.
+
+Section StuckTid.
+  Context `{EqDecision (locale Λ)}.
+
+(* TODO: move all of this *)
+  Definition not_stuck_tid (τ: locale Λ) (c: cfg Λ) :=
+    exists e, from_locale c.1 τ = Some e /\ not_stuck e c.2.
+
+  Definition stuck_tid τ c :=
+    exists e, from_locale c.1 τ = Some e /\ stuck e c.2.
+
+  Lemma stuck_tid_neg τ c:
+    ¬ not_stuck_tid τ c /\ is_Some (from_locale c.1 τ) <-> stuck_tid τ c.
+  Proof using.
+    rewrite /not_stuck_tid /stuck_tid.
+    setoid_rewrite <- not_not_stuck. 
+    split.
+    - intros (?&(?&?)). eexists. split; eauto.  
+    - intros (?&?&?). split; eauto.
+      intros (?&?&?). edestruct H0; eauto. congruence.   
+  Qed.
+    
+  (* TODO: is it provable for general Λ? *)
+  Global Instance not_stuck_dec e (c: language.state Λ): Decision (not_stuck e c).
+  Proof using.
+    rewrite /not_stuck.
+    apply or_dec; try solve_decision.
+    rewrite /reducible.
+  Admitted. 
+
+  Global Instance not_stuck_tid_dec `{EqDecision (expr Λ)} τ c: Decision (not_stuck_tid τ c).
+  Proof using.
+    rewrite /not_stuck_tid.
+    destruct (from_locale c.1 τ) as [e| ] eqn:TT.
+    2: right; by intros (?&?&?).
+    destruct (decide (not_stuck e c.2)).
+    - left. eauto.
+    - right; intros (?&?&?). congruence.
+  Qed.
+
+End StuckTid.
 
 
 Section TraceContext.
