fairness/utils_lists.v
@@ -1,0 +1,61 @@
+From stdpp Require Import base.
+From iris.proofmode Require Import tactics.
+
+Lemma fmap_flat_map {A B C: Type} (f : A → list B) (g: B -> C) (l : list A):
+  g <$> (flat_map f l) = flat_map ((fmap g) ∘ f) l.
+Proof.
+  induction l; [done| ].
+  simpl. rewrite fmap_app. congruence.
+Qed.
+
+Lemma concat_NoDup {A: Type} (ll : list (list A)):
+  (forall i l, ll !! i = Some l -> NoDup l) ->
+  (forall i j li lj, i ≠ j -> ll !! i = Some li -> ll !! j = Some lj -> li ## lj) ->
+  NoDup (concat ll).
+Proof.
+  induction ll.
+  { constructor. }
+  intros. simpl. apply NoDup_app. repeat split.
+  { apply (H 0). done. }
+  2: { apply IHll.
+       - intros. apply (H (S i)). done.
+       - intros. apply (H0 (S i) (S j)); auto. }
+  intros. intros [lx [INlx INx]]%elem_of_list_In%in_concat.
+  apply elem_of_list_In, elem_of_list_lookup_1 in INlx as [ix IX].
+  eapply (H0 0 (S ix)).
+  - lia.
+  - simpl. reflexivity.
+  - simpl. apply IX.
+  - eauto.
+  - by apply elem_of_list_In.
+Qed.
+
+(* TODO: find existing*)
+Lemma nth_error_lookup {A: Type} (l: list A) i:
+  nth_error l i = l !! i.
+Proof using.
+  rewrite /lookup. 
+  generalize dependent i. induction l.
+  { simpl. intros. by destruct i. }
+  intros. destruct i; try done. simpl. eauto.
+Qed.
+
+Lemma zip_lookup_Some_1 {A B: Type} (la: list A) (lb: list B) i a b:
+  zip la lb !! i = Some (a, b) -> la !! i = Some a /\ lb !! i = Some b.
+Proof using.
+  clear. 
+  revert la lb a b. induction i.
+  { intros. destruct la, lb; simpl in *; try discriminate. set_solver. }
+  intros. destruct la, lb; simpl in *; try discriminate.
+  apply IHi in H. done.
+Qed.
+
+Lemma foldl_foldr_rev {A B : Type} (f : B → A → B) (b : B) (la : list A):
+  foldl f b la = foldr (flip f) b (rev la). 
+Proof using.
+  generalize dependent b. induction la.
+  { done. }
+  simpl. intros. rewrite IHla.
+  by rewrite foldr_app.
+Qed.
+
