lawyer/nonblocking/examples/list_map_adequacy.v
@@ -1,30 +1,6 @@
 From heap_lang Require Import lang notation.
 From lawyer.nonblocking Require Import counter list_map wfree_adequacy wfree_traces.
 
-
-(* TODO: move *)
-Lemma always_returns_impl m etr s1 s2
-  (S12: stuckness_le s1 s2)
-  :
-  always_returns m s1 etr -> always_returns m s2 etr.
-Proof using.
-  rewrite /always_returns. simpl.
-  intros AR [i tpc] **.
-  ospecialize * (AR (trace_context.TraceCtx i tpc)); eauto.
-  destruct AR as [| (->&?)]; [by left| ].
-  destruct s2; try done. by right.
-Qed.
-
-(* TODO: move *)
-Lemma wait_free_impl m C1 C2 s1 s2
-  (C21: forall c, C2 c -> C1 c)
-  (S12: stuckness_le s1 s2):
-  wait_free m C1 s1 -> wait_free m C2 s2.
-Proof using.
-  From trillium.traces Require Import inftraces exec_traces. 
-  rewrite /wait_free. simpl. intros WF ? INIT ??.
-  eapply always_returns_impl; eauto.
-Qed.
   
 
 Theorem list_map_incr_is_wait_free
