lawyer/nonblocking/examples/pwp_tactics.v
@@ -1,0 +1,19 @@
+From iris.proofmode Require Import proofmode coq_tactics tactics.
+From heap_lang Require Import lang.
+From lawyer Require Import program_logic.
+From lawyer.nonblocking Require Import pwp.
+
+
+Ltac solve_vcs := 
+  match goal with
+    |- vals_compare_safe ?x ?y => red; set_solver
+  end. 
+
+Ltac pwp_pure_step :=
+    try (iEval (rewrite /pwp));
+    try (iApply trillium.program_logic.weakestpre.wp_value; []);
+    try (wp_bind (Rec _ _ _)%E || wp_bind (App _ _)%E);
+    (iApply sswp_pwp; [done| ]; iApply sswp_pure_step; (try solve_vcs || done); [ ]; do 2 iModIntro; iEval (simpl) );
+    try (iApply trillium.program_logic.weakestpre.wp_value; [] || iEval (rewrite /pwp)). 
+
+Ltac pwp_pure_steps := repeat pwp_pure_step. 
