lawyer/nonblocking/tokens/pwp_ext.v
@@ -29,6 +29,23 @@ Section CallTracker.
   Definition ct_auth (oe: option expr) := own ct_γ $ ● (Some $ Excl oe).
   Definition ct_frag (oe: option expr) := own ct_γ $ ◯ (Some $ Excl oe).
 
+  Lemma ct_auth_frag_agree c1 c2:
+    ct_auth c1 -∗ ct_frag c2 -∗ ⌜ c2 = c1 ⌝. 
+  Proof using.
+    simpl.
+    rewrite bi.wand_curry -own_op.
+    iIntros "X". iDestruct (own_valid with "[$]") as %V.
+    iPureIntro. symmetry. by apply excl_auth_agree_L.
+  Qed.  
+
+  Lemma ct_auth_frag_update c1 c2 c':
+    ct_auth c1 -∗ ct_frag c2 ==∗ ct_auth c' ∗ ct_frag c'. 
+  Proof using.
+    simpl. 
+    rewrite bi.wand_curry -!own_op.
+    iApply own_update. apply excl_auth_update. 
+  Qed.
+
 End CallTracker.
 
 
@@ -49,6 +66,87 @@ Section PwpExtra.
       (forall j, i <= j <= last_ind -> from_option (nval_at κ) False (etr !! j)) /\
       from_option (fun eτ => under_ctx K eτ = Some e) False ((trace_last etr).1 !! τ)
   . 
+
+  Lemma inside_call_extend extr tp1 tp2 K e σ1
+    (Hζ : locale_of tp1 (fill K e) = τ)
+    (Hextr : trace_ends_in extr (tp1 ++ fill K e :: tp2, σ1))
+    (s : nat)
+    (CALL : inside_call K s extr e)
+    (e2 : expr)
+    (σ2 : state)
+    (STEP : ectx_language.prim_step e σ1 e2 σ2 [])
+    (V2 : to_val e2 = None):
+    inside_call K s (extr :tr[ Some τ ]: (tp1 ++ fill K e2 :: tp2 ++ [], σ2)) e2.
+  Proof using.
+    red in CALL. destruct CALL as (a & CALL & PREV & NORET & CUR).
+    pose proof (trace_length_at_least extr) as LENnz. simpl in LENnz.
+    remember (trace_length extr) as N.
+    red. exists a. simpl. rewrite -HeqN. rewrite -HeqN in LENnz PREV.
+     repeat split.
+    - destruct CALL as (?&CALL&?). eexists. split; eauto.
+      rewrite -CALL. apply trace_lookup_extend_lt. rewrite -HeqN. lia.
+    - lia.
+    - simpl. intros j DOM.
+      assert (s <= j <= trace_length extr - 1 \/ j = trace_length extr) as [DOM' | ->].
+      { lia. }
+      + pose proof DOM' as X%NORET. 
+        destruct (extr !! j) eqn:JTH; rewrite JTH /= in X; [| done].
+        rewrite trace_lookup_extend_lt.
+        2: { rewrite -HeqN. lia. }
+        rewrite JTH. eauto.
+      + rewrite trace_lookup_last.
+        2: { simpl. rewrite -HeqN. lia. }
+        simpl.
+        red. eexists. split; [| apply V2]. 
+        red.
+        rewrite -Hζ. rewrite /from_locale.
+        by rewrite from_locale_from_locale_of.
+    - rewrite app_nil_r.
+      rewrite -Hζ. rewrite /locale_of.
+      rewrite list_lookup_middle; [| done].
+      simpl. by apply under_ctx_spec.
+  Qed. 
+
+  Lemma bump_inside_call K s0 e τ' c'' etr
+    (OTHER: τ' ≠ τ)
+    (CALL: inside_call K s0 etr e)
+    (STEP: locale_step (trace_last etr) (Some τ') c'')
+    :
+  inside_call K s0 (etr :tr[ Some τ' ]: c'') e.
+  Proof using.
+    clear -CALL STEP OTHER.
+    unfold inside_call in *.
+    destruct CALL as (a & CALL & PREV & NORET & CUR).
+    exists a. repeat split.
+    - destruct CALL as (?&?&?).
+      eexists. split; eauto. rewrite -H.
+      apply trace_lookup_extend_lt. lia.
+    - simpl in *. lia.
+    - simpl. rewrite Nat.sub_0_r.
+      intros j [GE LE]. apply Nat.le_lteq in LE as [LT | ->].
+      { simpl in *. specialize (NORET j ltac:(lia)).
+        destruct (etr !! j) eqn:JTH; [| done].
+        rewrite trace_lookup_extend_lt; [| done].
+        by rewrite JTH. }
+      rewrite trace_lookup_extend /=; [| done].
+      specialize (NORET (trace_length etr -1) ltac:(lia)).
+      destruct (etr !! (trace_length etr - 1)) eqn:LAST; [| done]. simpl in *.
+      rewrite trace_lookup_last in LAST.
+      2: simpl; lia.
+      inversion LAST. subst c.
+      destruct NORET as (?&?&?). simpl in *.
+      eapply locale_step_other_same in STEP; eauto.
+      2: congruence.
+      red. eauto.
+    - simpl.
+      destruct ((trace_last etr).1 !! τ) eqn:TT; [| done]. simpl in *.
+      apply under_ctx_spec in CUR. subst. 
+      eapply locale_step_other_same in STEP; eauto.
+      2: { apply from_locale_lookup. eauto. }
+      2: congruence.
+      apply from_locale_lookup in STEP. rewrite STEP /=.
+      eapply under_ctx_spec; eauto.
+  Qed.
 
   Context (tok: iProp Σ).
 
